Cminorgen proof 95%complete, and associated tweakings of effects etc

sepcomp/effect_semantics.v
@@ -12,25 +12,26 @@ Require Import sepcomp.mem_lemmas. (*needed for definition of mem_forward etc*)
 Require Import sepcomp.core_semantics.
 Require Import sepcomp.StructuredInjections.
 
+Lemma unch_on_validblock: forall m m' (U V: Values.block -> Z -> Prop)
+   (UV: forall b ofs, Mem.valid_block m b -> (U b ofs -> V b ofs)),
+   Mem.unchanged_on V m m' -> Mem.unchanged_on U m m'.
+  Proof. intros.
+    destruct H.
+    split; intros. 
+       eapply unchanged_on_perm; try eassumption. eauto.
+       eapply unchanged_on_contents; try eassumption. 
+       apply Mem.perm_valid_block in H0. eauto.
+Qed.
+
 Lemma unch_on_validblock_invariant: forall m m' U V
    (UV: forall b ofs, Mem.valid_block m b -> (U b ofs <-> V b ofs)),
    Mem.unchanged_on V m m' <-> Mem.unchanged_on U m m'.
   Proof. intros.
-    split; intros Hyp; destruct Hyp.
     split; intros. 
-       eapply unchanged_on_perm; try eassumption.
-       destruct (UV _ ofs H0). eauto.
-
-       eapply unchanged_on_contents; try eassumption.
-       apply Mem.perm_valid_block in H0.
-       destruct (UV _ ofs H0). eauto.
-    split; intros. 
-       eapply unchanged_on_perm; try eassumption.
-       destruct (UV _ ofs H0). eauto.
-
-       eapply unchanged_on_contents; try eassumption.
-       apply Mem.perm_valid_block in H0.
-       destruct (UV _ ofs H0). eauto.
+       eapply unch_on_validblock; try eassumption.
+          intros. destruct (UV _ ofs H0). eauto.
+       eapply unch_on_validblock; try eassumption.
+          intros. destruct (UV _ ofs H0). eauto.
 Qed.
 
 Lemma unch_on_perm_intersection: forall m m' U (Fwd: mem_forward m m'),
@@ -55,16 +56,43 @@ Lemma unch_on_perm_intersection: forall m m' U (Fwd: mem_forward m m'),
         eapply Mem.perm_implies. eapply Mem.perm_max; eassumption. 
                apply perm_any_N.
 Qed.
+
+
+Lemma mem_unchanged_on_trans: forall m1 m2 m3 U
+      (U1: Mem.unchanged_on U m1 m2) 
+      (U2: Mem.unchanged_on U m2 m3)
+      (Fwd12: mem_forward m1 m2),
+  Mem.unchanged_on U m1 m3.
+Proof. intros.
+split; intros.
+  split; intros.
+    eapply U2; trivial. apply Fwd12; trivial.
+    eapply U1; trivial.
+  eapply U1; trivial. eapply U2; trivial. apply Fwd12; trivial.
+destruct U1 as [P1 V1]; destruct U2 as [P2 V2].
+  rewrite (V2 _ _ H).
+    apply V1; trivial.
+  apply P1; trivial. eapply Mem.perm_valid_block; eassumption.
+Qed.
  
 Record EffectSem {G C} :=
   { sem :> CoopCoreSem G C;
 
     effstep: G -> (block -> Z -> bool) -> C -> mem -> C -> mem -> Prop;
 
-    effax: forall M g c m c' m',
-       effstep g M c m c' m' <->
+    effax1: forall M g c m c' m',
+       effstep g M c m c' m' ->
             corestep sem g c m c' m'  
-         /\ Mem.unchanged_on (fun b ofs => M b ofs = false) m m'
+         /\ Mem.unchanged_on (fun b ofs => M b ofs = false) m m';
+
+    effax2: forall g c m c' m',
+       corestep sem g c m c' m' ->
+       exists M, effstep g M c m c' m';
+
+    effstep_sub_val: forall g U V c m c' m'
+         (UV: forall b ofs, Mem.valid_block m b -> 
+              U b ofs = true -> V b ofs = true),
+         effstep g U c m c' m' -> effstep g V c m c' m'
  }.
 
 Section effsemlemmas.
@@ -81,16 +109,16 @@ Qed.
 Lemma effstep_corestep: forall M g c m c' m',
       effstep Sem g M c m c' m' -> corestep Sem g c m c' m'. 
 Proof. intros.
-  apply effax in H. apply H.
+  apply effax1 in H. apply H.
 Qed.
 
 Lemma effstep_unchanged: forall M g c m c' m',
       effstep Sem g M c m c' m' -> 
       Mem.unchanged_on (fun b ofs => M b ofs = false) m m'.
 Proof. intros.
-  apply effax in H. apply H.
+  apply effax1 in H. apply H.
 Qed.
-
+(*
 Lemma effstep_rev: forall M g c m c' m',
       corestep Sem g c m c' m' ->
       Mem.unchanged_on (fun b ofs => M b ofs = false) m m' ->
@@ -100,29 +128,19 @@ Proof. intros.
   apply effax. 
   split; trivial.
 Qed.
-
+*)
   Lemma effstep_fwd: forall U c m c' m',
     effstep Sem g U c m c' m' -> mem_forward m m'.
   Proof. intros. destruct Sem.
-         eapply corestep_fwd. eapply effax. apply H.
+         eapply corestep_fwd. eapply effax1. apply H.
   Qed.
 
 Lemma effstep_sub: forall U V c m c' m'
          (UV: forall b ofs, U b ofs = true -> V b ofs = true),
          (effstep Sem g U c m c' m' -> effstep Sem g V c m c' m').
-Proof. intros. rewrite effax; rewrite effax in H.
-  destruct H as [CS Unch].
-      split; trivial.
-      split; intros; eapply Unch; trivial.
-       remember (U b ofs) as d.
-       destruct d; trivial; apply eq_sym in Heqd.
-       rewrite (UV _ _ Heqd) in H. assumption.
-
-       remember (U b ofs) as d.
-       destruct d; trivial; apply eq_sym in Heqd.
-       rewrite (UV _ _ Heqd) in H. assumption.
+Proof. intros. eapply (effstep_sub_val _ _ U V). intuition. assumption.
 Qed.
-
+(*
 Lemma effstep_sub_val: forall U V c m c' m'
          (UV: forall b ofs, Mem.valid_block m b -> U b ofs = true -> V b ofs = true),
          (effstep Sem g U c m c' m' -> effstep Sem g V c m c' m').
@@ -139,7 +157,7 @@ Proof. intros. rewrite effax; rewrite effax in H.
           apply Mem.perm_valid_block in H0.
           rewrite (UV _ _ H0 Heqd) in H. inv H.
 Qed.
-         
+*)         
 (*
 Record EffectSem {G C} :=
   { sem :> CoopCoreSem G C;
@@ -625,13 +643,13 @@ Qed.
     exists n. eapply effstepN_sub_val; eassumption.
   Qed. 
 
-  Lemma effstep_star_sub_val: forall c m c' m' (U V : block -> Z -> bool),
-     effstep_plus U c m c' m' ->
+  Lemma effstep_star_sub_val: forall c m c' m' (U : block -> Z -> bool)
+     (EFF: effstep_star U c m c' m') (V : block -> Z -> bool),
      (forall b z, Mem.valid_block m b -> U b z = true -> V b z = true) ->
      effstep_star V c m c' m'.
   Proof. intros.
-    destruct H as [n H].
-    exists (S n). eapply effstepN_sub_val; eassumption.
+    destruct EFF as [n EFF].
+    exists n. eapply effstepN_sub_val; eassumption.
   Qed. 
 (*
   Lemma effstep_sub_valid: forall c m c' m' (U V : block -> Z -> bool),
@@ -962,687 +980,135 @@ Qed.
 *)
 
 End effsemlemmas.
-(*
-Definition join (j k:meminj):meminj := fun b =>
-  match j b with
-     Some (b1, delta) => Some (b1,delta)
-   | None => k b
+
+
+Definition EmptyEffect: Values.block -> Z -> bool := fun b z => false.
+
+Lemma EmptyEffect_alloc: forall m lo hi m' b (ALLOC: Mem.alloc m lo hi = (m', b)),
+      Mem.unchanged_on (fun b ofs => EmptyEffect b ofs = false) m m'.
+Proof. intros.
+       eapply Mem.alloc_unchanged_on; eassumption.
+Qed. 
+
+Definition FreeEffect m lo hi (sp b:Values.block) (ofs:Z): bool := 
+   if valid_block_dec m b 
+   then eq_block b sp && zle lo ofs && zlt ofs hi
+   else false.
+
+Lemma FreeEffect_free: forall m sp lo hi m'
+             (FREE: Mem.free m sp lo hi = Some m'),
+     Mem.unchanged_on  (fun b ofs => FreeEffect m lo hi sp b ofs = false) m m'.
+Proof. intros.
+       eapply Mem.free_unchanged_on; try eassumption.
+               intros. unfold FreeEffect; simpl. intros N.
+               destruct (valid_block_dec m sp).
+               apply andb_false_iff in N. destruct H.
+               destruct (eq_block sp sp); simpl in *.
+                 destruct N. destruct (zle lo i). inv H1. xomega.
+               destruct (zlt i hi). inv H1. xomega.
+               apply n; trivial.
+               apply Mem.free_range_perm in FREE.
+                 apply n; clear n.
+                 eapply Mem.perm_valid_block.
+                 eapply (FREE lo). omega.
+Qed. 
+
+Definition FreelistEffect m (L: list (Values.block * Z * Z)) (b:Values.block) (ofs:Z): bool := 
+  List.fold_right (fun X E b z => match X with (bb,lo,hi) =>
+                                   E b z || FreeEffect m lo hi bb b z
+                                 end) 
+                 EmptyEffect L b ofs.
+
+Lemma FreelistEffect_Dfalse: forall m bb lo hi L b ofs
+      (F:FreelistEffect m ((bb, lo, hi) :: L) b ofs = false),
+      FreelistEffect m L b ofs = false /\
+      FreeEffect m lo hi bb b ofs = false. 
+Proof. intros.
+  unfold FreelistEffect in F. simpl in F.
+  apply orb_false_iff in F. apply F.
+Qed. 
+
+Lemma FreelistEffect_Dtrue: forall m bb lo hi L b ofs
+      (F:FreelistEffect m ((bb, lo, hi) :: L) b ofs = true),
+      FreelistEffect m L b ofs = true \/
+      FreeEffect m lo hi bb b ofs = true.
+Proof. intros.
+  unfold FreelistEffect in F. simpl in F.
+  apply orb_true_iff in F. apply F.
+Qed. 
+
+Lemma FreelistEffect_same: forall m bb lo hi mm L
+          (F:Mem.free m bb lo hi = Some mm)
+          b (VB: Mem.valid_block mm b) ofs,
+      FreelistEffect mm L b ofs = false <-> FreelistEffect m L b ofs = false.
+Proof. intros  m bb lo hi mm L.
+  induction L; simpl; intros. intuition.
+  intuition. 
+    apply orb_false_iff in H0. destruct H0.
+    specialize (H _ VB ofs).
+    apply H in H0. rewrite H0. simpl. clear H H0.
+    unfold FreeEffect in *; simpl in *.
+    apply Mem.nextblock_free in F. 
+    destruct (valid_block_dec m b). 
+      destruct (valid_block_dec mm b); trivial.
+      red in v. rewrite <- F in v. elim n. apply v.
+    trivial.
+  apply orb_false_iff in H0. destruct H0.
+    specialize (H _ VB ofs).
+    apply H in H0. rewrite H0. simpl. clear H H0.
+    unfold FreeEffect in *; simpl in *.
+    apply Mem.nextblock_free in F. 
+    destruct (valid_block_dec mm b). 
+      destruct (valid_block_dec m b); trivial.
+      red in v. rewrite F in v. elim n. apply v.
+    trivial.
+Qed.
+
+Lemma FreelistEffect_freelist: forall L m m' (FL: Mem.free_list m L = Some m'),
+      Mem.unchanged_on (fun b ofs => FreelistEffect m L b ofs = false) m m'.
+Proof. intros L.
+  induction L; simpl; intros.
+    inv FL. apply Mem.unchanged_on_refl.
+  destruct a as [[bb lo] hi].
+    remember (Mem.free m bb lo hi) as d.
+    destruct d; try inv FL. apply eq_sym in Heqd.
+    specialize (IHL _ _ H0).
+    assert (FF:= FreeEffect_free _ _ _ _ _ Heqd). 
+    eapply (mem_unchanged_on_trans _ m0 _).
+      eapply mem_unchanged_on_sub; try eassumption.
+        intuition. apply orb_false_iff in H. apply H.
+      clear FF.
+      specialize (unch_on_validblock_invariant m0 m' (fun (b : block) (ofs : Z) => FreelistEffect m0 L b ofs = false) (fun (b : block) (ofs : Z) => FreelistEffect m L b ofs = false)).
+      intros. apply H in IHL. clear H.
+        eapply mem_unchanged_on_sub; try eassumption.
+        intuition. apply orb_false_iff in H. apply H.
+      clear IHL H. intros.
+       eapply FreelistEffect_same; eassumption.
+   eapply free_forward; eassumption.
+Qed.
+
+Definition StoreEffect (tv:val)(vl : list memval) (b:Values.block) (z:Z):bool := 
+  match tv with Vptr bb ofs => eq_block bb b && 
+             zle (Int.unsigned ofs) z && zlt z (Int.unsigned ofs + Z.of_nat (length vl))
+         | _ => false
   end.
 
-Definition disjoint (j k:meminj):Prop :=
-    forall b, j b = None \/ k b = None.
-
-Lemma joinD: forall j k (D: disjoint j k) b,
-   match join j k b with
-     Some(b1,delta) => (j b = Some(b1,delta) /\ k b = None) \/
-                       (k b = Some(b1,delta) /\ j b = None)
-   | None => j b = None /\ k b = None
-  end.
+Lemma StoreEffect_Storev: forall m chunk tv tv' m' 
+         (STORE : Mem.storev chunk m tv tv' = Some m'),
+      Mem.unchanged_on (fun b ofs => StoreEffect tv (encode_val chunk tv') b ofs = false) m m'.
 Proof. intros.
-  unfold join. destruct (D b); rewrite H.
-     case_eq (k b); eauto.
-     destruct p; eauto.
-   case_eq (j b); eauto.
-     destruct p; eauto. 
+  destruct tv; inv STORE.
+  unfold StoreEffect.
+  split; intros.
+      split; intros. eapply Mem.perm_store_1; eassumption.
+      eapply Mem.perm_store_2; eassumption.
+  rewrite (Mem.store_mem_contents _ _ _ _ _ _ H0). clear H0.
+  destruct (eq_block b b0); subst; simpl in *.
+    rewrite PMap.gss. apply andb_false_iff in H.  
+    apply Mem.setN_outside.
+    destruct H. destruct (zle (Int.unsigned i) ofs ); simpl in *. inv H.
+                left. xomega.
+    right. remember (Z.of_nat (length (encode_val chunk tv'))).
+       destruct (zlt ofs (Int.unsigned i + z)); simpl in *. inv H. apply g.
+  rewrite PMap.gso. trivial. intros N; subst. elim n; trivial. 
 Qed.
-
-Record SM_Injection :=
-  { myBlocksSrc : block -> Prop;
-                     (* The blocks allocated by THIS module in the
-                        source language SRC*)
-    myBlocksTgt : block -> Prop; 
-                     (* The blocks allocated by THIS module in the
-                        target language TGT*)
-    frgnInj: meminj; (* a meminj on blocks allocated by other modules; 
-                        the injection itself is not modified by coresteps
-                        but blocks mentioned by it are accessible. THIS module
-                        behaves UNIFORMLY over block mentioned by frgnInj, and
-                        assumes that blocks in frgnInj remain mapped during
-                        "compilation of the environment". Compilation of THIS 
-                        module neither merges nor unmaps blocks from here, 
-                        not does it spill into them*)
-    pubInj: meminj; (* a meminj on blocks allocated by THIS module.
-                       This injection (and hence its constituent blocks) 
-                       is revealed to other modules in at_external and halted, 
-                       hence other modules may read from / write to blocks 
-                       mentioned here - but do so only in a UNIFORM manner.
-                       THIS module may spill into blocks mentioned here, but its
-                       compilation should not unmap blocks from here (since they
-                       have been revealed to other modules).*)
-    privInj: meminj; (* another meminj on blocks allocated by THIS module.
-                        This injection is entirely private: it is not revealed
-                        to other modules at at_external or halted,
-                        so blocks in here will necessarily remain unmodified 
-                        over external calls. Compilation of THIS module
-                        may arbitrarily unmap a block b from dom privinj 
-                        in some later phase. Compilation may also spill into 
-                        such a block, and may map it with a block
-                        b' from dom pubInj or dom privInj (but not frgnInj). 
-                        If b' is from pubInj, the resulting merged block b1 will 
-                        then necessarily be mapped by all later compilation phases,
-                        and is revealed at at_external and halted from TGT
-                        onwards (since b' already was revealed in SRC or earlier).
-                        However, even downstream from TGT, locations in b1 that
-                        "originate" from b remain unmodified across external calls,
-                        since the invoked module OTHER did not know about these
-                        locations in the SRC and behaves UNFORMLY
-                        over the locations in b'. In particular, foreign modules
-                        don't spill into b, b' or b1, while THIS module may
-                        safely spill into all three blocks. *)
-    dist : disjoint pubInj privInj;
-    localDOM: forall b1 b2 z, join pubInj privInj b1 = Some(b2,z) -> 
-               (myBlocksSrc b1 /\ myBlocksTgt b2);
-    foreignDOM: forall b1 b2 z, frgnInj b1 = Some(b2,z) -> 
-               (~myBlocksSrc b1 /\ ~myBlocksTgt b2)
-  }.
-
-
-(*DOM/RNG: all blocks mentioned by a SM_Injection. Used for
-  stating match_validblocks etc*)
-Definition DOM (X: SM_Injection) (b1: block): Prop.
-  destruct X as [BSrc BTgt frgn pub priv _ _ _]. 
-  apply (BSrc b1 \/ exists b2 z, frgn b1 = Some (b2,z)).
-Defined.
-  
-Definition RNG (X: SM_Injection) (b2:block): Prop.
-  destruct X as [BSrc BTgt frgn pub priv _ _ _].
-  apply (BTgt b2 \/ exists b1 z, frgn b1 = Some (b2,z)).
-Defined.
-
-(*The join of all three components - useful for stating
-  match_state conditions*)
-Definition as_inj (X: SM_Injection) : meminj.
-  destruct X as [BSrc BTgt frgn pub priv _ _ _].
-  apply (join frgn (join pub priv)).
-Defined.
-
-(*The three projections*)
-Definition foreign_of (X: SM_Injection) : meminj.
-  destruct X as [BSrc BTgt frgn pub priv _ _ _].
-  apply frgn.
-Defined.
-
-Definition pub_of (X: SM_Injection) : meminj.
-  destruct X as [BSrc BTgt frgn pub priv _ _ _].
-  apply pub.
-Defined.
-
-Definition priv_of (X: SM_Injection) : meminj.
-  destruct X as [BSrc BTgt frgn pub priv _ _ _].
-  apply priv.
-Defined.
-
-(*Two derived notions, local and shared*)
-Definition local_of (X: SM_Injection) : meminj.
-  destruct X as [BSrc BTgt frgn pub priv _ _ _].
-  apply (join pub priv).
-Defined.
-
-Definition shared_of (X: SM_Injection) : meminj.
-  destruct X as [BSrc BTgt frgn pub priv _ _ _].
-  apply (join frgn pub).
-Defined.
-
-(*Obvious incject_incr relationships*)
-Lemma pub_in_local: forall j, inject_incr (pub_of j) (local_of j).
-Proof. intros.
-  destruct j as [BSrc BTgt frgn pub priv dst locDom frgnDom]; simpl in *.
-  intros b1; intros.
-  unfold join. rewrite H. trivial.
-Qed.
-
-Lemma priv_in_local: forall j, inject_incr (priv_of j) (local_of j).
-Proof. intros.
-  destruct j as [BSrc BTgt frgn pub priv dst locDom frgnDom]; simpl in *.
-  intros b1; intros.
-  unfold join. rewrite H.
-  case_eq (pub b1); intros; trivial.
-  destruct p. 
-  destruct (dst b1) as [D | D]; rewrite D in *; congruence. 
-Qed.
-
-Lemma local_in_all: forall j, inject_incr (local_of j) (as_inj j).
-Proof. intros.
-  destruct j as [BSrc BTgt frgn pub priv dst locDom frgnDom]; simpl in *.
-  intros b1; intros.
-  destruct (locDom _ _ _ H).
-  unfold join in *. rewrite H.
-  case_eq (frgn b1); intros; trivial.
-  destruct p. destruct (frgnDom _ _ _ H2); contradiction.
-Qed.
-
-Lemma pub_in_all: forall j, inject_incr (pub_of j) (as_inj j).
-Proof. intros.
-  eapply inject_incr_trans.
-  apply pub_in_local. apply local_in_all.
-Qed.
-
-Lemma priv_in_all: forall j, inject_incr (priv_of j) (as_inj j).
-Proof. intros.
-  eapply inject_incr_trans.
-  apply priv_in_local. apply local_in_all.
-Qed.
-
-Lemma pub_in_shared: forall j, inject_incr (pub_of j) (shared_of j).
-Proof. intros.
-  destruct j as [BSrc BTgt frgn pub priv dst locDom frgnDom]; simpl in *.
-  intros b1; intros.
-  unfold join. rewrite H.
-  case_eq (frgn b1); intros; trivial.
-  destruct p.
-  destruct (frgnDom _ _ _ H0).
-  exfalso. apply H1.
-  apply (locDom b1 b' delta). 
-  unfold join. rewrite H. trivial.
-Qed.
-
-Lemma foreign_in_shared: forall j, inject_incr (foreign_of j) (shared_of j).
-Proof. intros.
-  destruct j as [BSrc BTgt frgn pub priv dst locDom frgnDom]; simpl in *.
-  intros b1; intros.
-  unfold join. rewrite H. trivial.
-Qed.
-
-Lemma shared_in_all: forall j, inject_incr (shared_of j) (as_inj j).
-Proof. intros.
-  destruct j as [BSrc BTgt frgn pub priv dst locDom frgnDom]; simpl in *.
-  intros b1; intros.
-  unfold join in *.
-  remember (frgn b1) as d; destruct d; intros.
-    destruct p. apply H.
-  rewrite H. trivial.
-Qed.
-
-Lemma foreign_in_all: forall j, inject_incr (foreign_of j) (as_inj j).
-Proof. intros.
-  eapply inject_incr_trans.
-  apply foreign_in_shared. 
-  apply shared_in_all.
-Qed.
-
-(*Construction used in make_initial_core: put incoming injection
-  into foreign component, initialize the other componenet as empty*)
-Definition initial_SM (j: meminj) : SM_Injection.
-eapply Build_SM_Injection with (myBlocksSrc:=fun b => False)
-  (myBlocksTgt:=fun b => False) (frgnInj:=j) 
-  (privInj:=fun b => None)(pubInj:=fun b => None).
-intros b; intros; auto.
-intros. inv H.
-intros. auto.
-Defined.
-
-Definition sm_inject_incr (j j' : SM_Injection):Prop.
-destruct j as [BSrc BTgt frgn pub priv dst locDom frgnDom].
-destruct j' as [BSrc' BTgt' frgn' pub' priv' dst' locDom' frgnDom'].
-apply (inject_incr frgn frgn' /\ inject_incr pub pub' /\ 
-       inject_incr priv priv' /\
-       (forall b, BSrc b -> BSrc' b) /\
-       (forall b, BTgt b -> BTgt' b)).
-Defined.
-
-Definition sm_inject_separated (j j' : SM_Injection) (m1 m2:mem):Prop.
-destruct j as [BSrc BTgt frgn pub priv dst locDom frgnDom].
-destruct j' as [BSrc' BTgt' frgn' pub' priv' dst' locDom' frgnDom'].
-apply (inject_separated frgn frgn' m1 m2 /\ 
-       inject_separated pub pub' m1 m2 /\ 
-       inject_separated priv priv' m1 m2 /\
-       (forall b, ~BSrc b -> BSrc' b -> ~ Mem.valid_block m1 b) /\
-       (forall b, ~BTgt b -> BTgt' b -> ~ Mem.valid_block m2 b)).
-Defined.
-
-Definition sm_valid (j : SM_Injection) (m1 m2: mem) :=
-       (forall b1, DOM j b1 -> Mem.valid_block m1 b1)  
-    /\ (forall b2, RNG j b2 -> Mem.valid_block m2 b2).
-
-Definition extend_foreign (mu: SM_Injection)(j:meminj) (m1 m2:mem)
-           (INC: inject_incr (shared_of mu) j)  
-           (SEP: inject_separated (shared_of mu) j m1 m2)
-           (VB: sm_valid mu m1 m2) : SM_Injection.
-destruct mu as [BSrc BTgt frgn pub priv dst locDom frgnDom].
-eapply Build_SM_Injection with (myBlocksSrc:=BSrc)
-  (myBlocksTgt:=BTgt)
-  (frgnInj:=fun b => match pub b with 
-                       Some p => None
-                     | None => j b end)
-  (pubInj:=pub)
-  (privInj:=priv); trivial.
-destruct VB as [Dom Rng].
-intros; simpl in *.
-  remember (pub b1) as d.
-  destruct d; apply eq_sym in Heqd.
-    inv H.
-  remember (frgn b1) as q.
-    destruct q; apply eq_sym in Heqq.
-      destruct p. 
-      assert (j b1 = Some(b, z0)).
-        apply INC. unfold join. rewrite Heqq. trivial.
-      rewrite H0 in H. inv H. 
-      apply (frgnDom _ _ _ Heqq).
-    assert (join frgn pub b1 = None).
-      unfold join. rewrite Heqq. rewrite Heqd. trivial.
-    destruct (SEP _ _ _ H0 H).
-    split; intros N.
-      apply H1. apply Dom. left; trivial.
-      apply H2. apply Rng. left; trivial.
-Defined.
-
-Lemma extend_foreign_prop: forall mu j m1 m2
-           (INC: inject_incr (shared_of mu) j)  
-           (SEP: inject_separated (shared_of mu) j m1 m2)
-           (VB: sm_valid mu m1 m2) ,
-   (forall b1 b2 delta, (shared_of mu) b1 = Some(b2,delta) <-> 
-          ((as_inj mu) b1 = Some(b2,delta) /\ j b1 = Some(b2,delta)))
-   /\ inject_separated (as_inj mu) j m1 m2
-   /\ sm_inject_incr mu (extend_foreign _ _ _ _ INC SEP VB)
-   /\ sm_inject_separated mu (extend_foreign _ _ _ _ INC SEP VB) m1 m2.
-Proof.
-  intros.
-  destruct mu as [BSrc BTgt frgn pub priv dst locDom frgnDom].
-  simpl in *.
-  unfold extend_foreign in *; simpl in *.
-  split.
-  (*first prop*)
-    intros.
-    split; intros.
-      split. unfold join. unfold join in H. 
-           remember (frgn b1) as d.
-           destruct d. destruct p. trivial.
-           rewrite H. trivial.
-          apply INC; trivial.
-      destruct H.
-        unfold join in H. unfold join. 
-        remember (frgn b1) as d. 
-        destruct d; apply eq_sym in Heqd. 
-             destruct p. trivial.
-        remember (pub b1) as q.
-        destruct q. destruct p. trivial.
-        assert (join frgn pub b1 = None).
-           unfold join. rewrite Heqd. rewrite Heqq; trivial.
-        destruct (SEP _ _ _ H1 H0).
-          destruct VB. 
-         exfalso. apply H2. apply H4. simpl.  
-           left. eapply locDom. unfold join. 
-            rewrite H. rewrite <- Heqq. reflexivity.
-   (*second prop*)
-     split.
-       intros b1; intros.
-       assert (join frgn pub b1 = None).
-         unfold join; unfold join in H.
-         remember (frgn b1) as d.
-         destruct d. destruct p. inv H.
-         remember (pub b1) as q.
-         destruct q. destruct p. inv H. trivial.
-       apply (SEP _ _ _ H1 H0).
-  split. split.
-  (*third prop*)
-      intros b1; intros.
-      destruct (frgnDom _ _ _ H).
-      remember (pub b1) as d.
-      destruct d.
-        apply eq_sym in Heqd.
-        destruct p.
-        destruct (locDom b1 b z).
-          unfold join. rewrite Heqd. trivial.
-          contradiction.
-        apply INC. unfold join. rewrite H. trivial. 
-    split. apply inject_incr_refl. 
-    split. apply inject_incr_refl.
-    split; trivial.
-  split. intros b1; intros.
-    remember (pub b1) as d.
-    destruct d; apply eq_sym in Heqd.
-      inv H0.
-    apply (SEP b1 b2 delta); trivial.
-      unfold join. rewrite Heqd. rewrite H. trivial.
-  split. apply inject_separated_same_meminj.
-  split. apply inject_separated_same_meminj.
-  split; intuition.
-Qed.
-        
-
-Module SM_simulation. Section SharedMemory_simulation_inject. 
-  Context {F1 V1 C1 G2 C2:Type}
-          {Sem1 : @EffectSem (Genv.t F1 V1) C1}
-          {Sem2 : @EffectSem G2 C2}
-          {ge1: Genv.t F1 V1}
-          {ge2: G2}
-          {entry_points : list (val * val * signature)}.
-
-  Record SM_simulation_inject := 
-  { core_data : Type;
-    match_state : core_data -> SM_Injection -> C1 -> mem -> C2 -> mem -> Prop;
-    core_ord : core_data -> core_data -> Prop;
-    core_ord_wf : well_founded core_ord;
-
-    (*Same as for coop-simulations*)
-    match_memwd: forall d j c1 m1 c2 m2,
-          match_state d j c1 m1 c2 m2 -> 
-               (mem_wd m1 /\ mem_wd m2);
-
-    match_validblocks: forall d j c1 m1 c2 m2, 
-          match_state d j c1 m1 c2 m2 ->
-          sm_valid j m1 m2;               
-
-    (*External knowledge is put into pub component*)
-    core_initial : forall v1 v2 sig,
-       In (v1,v2,sig) entry_points -> 
-       forall vals1 c1 m1 j vals2 m2,
-          initial_core Sem1 ge1 v1 vals1 = Some c1 ->
-          Mem.inject j m1 m2 -> 
-          mem_wd m1 -> mem_wd m2 ->
-
-          Forall2 (val_inject j) vals1 vals2 ->
-
-          Forall2 (Val.has_type) vals2 (sig_args sig) ->
-          exists cd, exists c2, 
-            initial_core Sem2 ge2 v2 vals2 = Some c2 /\
-            match_state cd (initial_SM j) c1 m1 c2 m2;
-
-(*Here we distinguish beween "our" and "foreign" block*)
-    core_diagram : 
-      forall st1 m1 st1' m1', 
-        corestep Sem1 ge1 st1 m1 st1' m1' ->
-      forall cd st2 mu m2,
-        match_state cd mu st1 m1 st2 m2 ->
-        exists st2', exists m2', exists cd', exists mu',
-          sm_inject_incr mu mu' /\
-          sm_inject_separated mu mu' m1 m2 /\
-          (*new condition: corestep evolution only adds to local knowledge*)
-          foreign_of mu = foreign_of mu' /\ 
-          match_state cd' mu' st1' m1' st2' m2' /\
-          ((corestep_plus Sem2 ge2 st2 m2 st2' m2') \/
-            corestep_star Sem2 ge2 st2 m2 st2' m2' /\
-            core_ord cd' cd);
-(*TODO: replace these coresteps by appropriate effsteps, and/or add unchOn conditions*)
-
-    (*Only the shared part is revealed to the environment*)
-    core_halted : forall cd mu c1 m1 c2 m2 v1,
-      match_state cd mu c1 m1 c2 m2 ->
-      halted Sem1 c1 = Some v1 ->
-      val_valid v1 m1 ->
-      exists v2, 
-        val_inject (shared_of mu) v1 v2 /\
-        halted Sem2 c2 = Some v2 /\
-        Mem.inject (shared_of mu) m1 m2 /\ val_valid v2 m2;
-        (*Maybe we should additionally require 
-            Mem.inject (as_inj mu) m1 m2 and
-            val_inject (as_inj mu) v1 v2) ? The latter presumably 
-            follows already using shared_in_all*)
-
-    core_at_external : 
-      forall cd mu c1 m1 c2 m2 e vals1 ef_sig,
-        match_state cd mu c1 m1 c2 m2 ->
-        at_external Sem1 c1 = Some (e,ef_sig,vals1) ->
-        (forall v1, In v1 vals1 -> val_valid v1 m1) ->
-        ( (*The old conditions*)
-            Mem.inject (as_inj mu) m1 m2 /\  (*maybe this can now be deleted?*)
-            meminj_preserves_globals ge1 (as_inj mu) /\ 
-            exists vals2, Forall2 (val_inject (as_inj mu)) vals1 vals2 /\ (*maybe this can now be deleted?*)
-            Forall2 (Val.has_type) vals2 (sig_args ef_sig) /\
-            at_external Sem2 c2 = Some (e,ef_sig,vals2) /\
-            (forall v2, In v2 vals2 -> val_valid v2 m2) /\
-
-          (*new conditions: the shared blocks are leaked to the environment -
-             this set must include at least all blocks mentioned by
-             the function arguments and the foreign blocks, and must
-             be closed under pointer derferencing and arithmetic*)
-             Mem.inject (shared_of mu) m1 m2 /\ (*In particular: no pointers from shared to priv or localunmapped  are allowed*)
-             Forall2 (val_inject (shared_of mu)) vals1 vals2 /\
-             meminj_preserves_globals ge1 (shared_of mu)); (*not sure this is needed ..*)
-
-    core_after_external:
-      forall cd mu st1 st2 m1 e vals1 ret1 m1' m2 m2' ret2 ef_sig,
-        Mem.inject (as_inj mu) m1 m2->
-      forall
-        (MS: match_state cd mu st1 m1 st2 m2),
-        at_external Sem1 st1 = Some (e,ef_sig,vals1) ->
-        (forall v1, In v1 vals1 -> val_valid v1 m1) ->
-        meminj_preserves_globals ge1 (as_inj mu) -> 
-
-      forall vals2, 
-        Mem.inject (shared_of mu) m1 m2 -> 
-        Forall2 (val_inject (shared_of mu)) vals1 vals2 -> 
-        meminj_preserves_globals ge1 (shared_of mu) ->
-
-      forall j'
-        (INC: inject_incr (shared_of mu) j')  
-        (SEP: inject_separated (shared_of mu) j' m1 m2), 
-        (*hence inject_separated (as_inj mu) j' m1 m2 holds*)
-
-        Mem.inject j' m1' m2' ->
-        val_inject j' ret1 ret2 ->
-
-         mem_forward m1 m1' -> 
-(*think about this later         Mem.unchanged_on (loc_unmapped j) m1 m1' ->
-         (forall b1 b2 delta ofs, priv b1 = Some(b2,delta) -> U1 b1 ofs) ->?? 
-         Mem.unchanged_on U1 m1 m1' ->*)
-
-         mem_forward m2 m2' -> 
-(*think about this later         Mem.unchanged_on (loc_out_of_reach j m1) m2 m2' ->
-         Mem.unchanged_on (fun b2 ofs => forall b1 delta, lk b <> Some(b2,delta)) m2 m2' ->
-         Mem.unchanged_on m2 m2' ->*)
-
-         Val.has_type ret2 (proj_sig_res ef_sig) -> 
-
-         mem_wd m1' -> mem_wd m2' -> 
-         val_valid ret1 m1' -> val_valid ret2 m2' ->
-
-        exists cd', exists st1', exists st2',
-          after_external Sem1 (Some ret1) st1 = Some st1' /\
-          after_external Sem2 (Some ret2) st2 = Some st2' /\
-        exists mu',
-          mu' = extend_foreign mu j' m1 m2 INC SEP (match_validblocks _ _ _ _ _ _ MS)
-
-          /\ (*here we combine old knowledge with new knowledge*)
-              match_state cd' mu' st1' m1' st2' m2' 
-
-           (*Some conditions that were in fact proven in 
-               lemma extends_foreign_prop:
-               The common part of mu and j' is exactly (shared_of mu):
-           /\ (forall b1 b2 delta, (shared_of mu) b1 = Some(b2,delta) <-> 
-                      ((as_inj mu) b1 = Some(b2,delta) /\ j' b1 = Some(b2,delta)))
-           /\ inject_separated (as_inj mu) j' m1 m2
-           /\ sm_inject_incr mu mu'
-           /\ sm_inject_separated mu mu' m1 m2*)
-}.
-
-End SharedMemory_simulation_inject. 
-
-Require Import sepcomp.forward_simulations_trans.
-Require Import Wellfounded.
-Require Import Relations.
-
-Definition compose_sm (j1 j2 : SM_Injection) : SM_Injection.
-destruct j1 as [pBL1 pub1 priv1 pBR1 Dist1 dP1].
-destruct j2 as [pBL2 pub2 priv2 pBR2 Dist2 dP2].
-eapply Build_SM_Injection with
-  (privBlocks1:=pBL1)
-  (privBlocks2:=pBR2)
-  (pubInj:=compose_meminj pub1 pub2)
-  (privInj:=compose_meminj priv1 (join pub2 priv2)).
-intros b1.
-  remember (compose_meminj pub1 pub2 b1) as d.
-  destruct d; try (left; reflexivity).
-  right. destruct p as [b3 z].
-  apply eq_sym in Heqd.
-  remember (compose_meminj priv1 (join pub2 priv2) b1) as q.
-  destruct q; try reflexivity.
-  destruct p as [a3 w].
-  apply eq_sym in Heqq.
-  destruct (compose_meminjD_Some _ _ _ _ _ Heqd)
-     as [b2 [d2 [d3 [PUB1 [PUB2 X]]]]]; subst.
-  destruct (compose_meminjD_Some _ _ _ _ _ Heqq)
-     as [a2 [w2 [w3 [PRIV1 [PP2 X]]]]]; subst.
-  clear Heqd Heqq.
-  destruct (Dist1 b1).
-    rewrite H in PUB1; congruence.
-    rewrite H in PRIV1; congruence.
-intros b1 b3 z H.  
-  destruct (compose_meminjD_Some _ _ _ _ _ H)
-     as [b2 [d2 [d3 [PRIV1 [PP2 X]]]]]; subst.
-  clear H.
-  split. eapply dP1. apply PRIV1.
-Section Eff_sim_trans.
-Context {F1 V1 C1 F2 V2 C2 F3 V3 C3:Type}
-        (Sem1 : @EffectSem (Genv.t F1 V1) C1)
-        (Sem2 : @EffectSem (Genv.t F2 V2) C2)
-        (Sem3 : @EffectSem (Genv.t F3 V3) C3)
-        (g1 : Genv.t F1 V1)
-        (g2 : Genv.t F2 V2)
-        (g3 : Genv.t F3 V3) 
-        epts12 epts23 epts13
-        (EPC : entrypoints_compose epts12 epts23 epts13).
-
-Theorem eff_sim_trans: forall 
-        (SIM12: @SM_simulation_inject _ _ _ _ _ Sem1 Sem2 g1 g2 epts12)
-        (SIM23: @SM_simulation_inject _ _ _ _ _ Sem2 Sem3 g2 g3 epts23),
-        @SM_simulation_inject _ _ _ _ _ Sem1 Sem3 g1 g3 epts13.
-Proof. (*follows structire of forward_simulations_ytrans.injinj*)
-  intros.
-  destruct SIM12 
-    as [core_data12 match_core12 core_ord12 core_ord_wf12 match_memwd12 
-      match_validblock12 core_diagram12 
-      core_initial12 core_halted12 core_at_external12 core_after_external12].  
-  destruct SIM23 
-    as [core_data23 match_core23 core_ord23 core_ord_wf23  match_memwd23 
-      match_validblock23 core_diagram23 
-      core_initial23 core_halted23 core_at_external23 core_after_external23].
-  eapply Build_SM_simulation_inject with
-    (core_ord := clos_trans _ (sem_compose_ord_eq_eq core_ord12 core_ord23 C2)).
-    (match_state := fun d j c1 m1 c3 m3 => 
-      match d with (d1,X,d2) => 
-        exists c2, exists m2, exists j1, exists j2, 
-          X=Some c2 /\ j = compose_sm j1 j2 /\
-          match_core12 d1 j1 c1 m1 c2 m2 /\ match_core23 d2 j2 c2 m2 c3 m3 
-      end).
- (*well_founded*)
-  eapply wf_clos_trans. eapply well_founded_sem_compose_ord_eq_eq; assumption.
- (*match_wd*) intros. rename c2 into c3.  rename m2 into m3. destruct d as [[d12 cc2] d23]. 
-  destruct H as [c2 [m2 [j12 [j23 [X [J [MC12 MC23]]]]]]]; subst.
-  split. apply (match_memwd12 _ _ _ _ _ _ MC12).
-  apply (match_memwd23 _ _ _ _ _ _ MC23).
- (*match_validblocks*) 
-  intros. rename c2 into c3.  rename m2 into m3. destruct d as [[d12 cc2] d23]. 
-  destruct H as [c2 [m2 [j12 [j23 [X [J [MC12 MC23]]]]]]]; subst.
-  apply compose_meminjD_Some in H0. 
-  destruct H0 as [b11 [ofs11 [ofs12 [Hb [Hb1 Hdelta]]]]]. 
-  split. eapply (match_validblock12 _ _ _ _ _ _ MC12); try eassumption.
-  eapply (match_validblock23 _ _ _ _ _ _ MC23); try eassumption.
- (*core_diagram*)
-  clear core_initial23  core_halted23 core_at_external23 core_after_external23 
-    core_initial12  core_halted12 core_at_external12 core_after_external12
-    EPC epts12 epts23 epts13.
-  intros. rename st2 into st3. rename m2 into m3.
-  destruct cd as [[d12 cc2] d23]. destruct H0 as [st2 [m2 [j12 [j23 [X [? [MC12 MC23]]]]]]]; subst.
-  eapply (diagram_injinj _ _ _ core_diagram12 _ _ _ core_diagram23 
-    match_validblock12 match_validblock23); try eassumption.
- (*initial_core*)
-  clear core_diagram23  core_halted23 core_at_external23 core_after_external23 
-    core_diagram12  core_halted12 core_at_external12 core_after_external12.
-  intros. rename m2 into m3. rename v2 into v3. rename vals2 into vals3. 
-  rewrite (EPC v1 v3 sig) in H. destruct H as [v2 [EP12 EP23]].
-  assert (HT: Forall2 Val.has_type vals1 (sig_args sig)). 
-  eapply forall_valinject_hastype; eassumption.
-  destruct (mem_wd_inject_splitL _ _ _ H1 H2) as [Flat1 XX]; rewrite XX.
-  assert (ValInjFlat1 := forall_val_inject_flat _ _ _ H1 _ _ H4).
-  destruct (core_initial12 _ _ _ EP12 _ _ _ _ _ _ H0 Flat1 H2 H2 ValInjFlat1 HT) 
-    as [d12 [c2 [Ini2 MC12]]].
-  destruct (core_initial23 _ _ _ EP23 _ _ _ _ _ _  Ini2 H1 H2 H3 H4 H5) 
-    as [d23 [c3 [Ini3 MC23]]].
-  exists (d12,Some c2,d23). exists c3. 
-  split; trivial. 
-  exists c2. exists m1. exists  (Mem.flat_inj (Mem.nextblock m1)). exists j. 
-  split; trivial. split; trivial. split; assumption.
- (*halted*)
-  intros. rename c2 into c3. rename m2 into m3.  
-  destruct cd as [[d12 cc2] d23]. destruct H as [c2 [m2 [j12 [j23 [X [Y [MC12 MC23]]]]]]]; subst. 
-  apply (core_halted12 _ _ _ _ _ _ _ MC12) in H0; try assumption. 
-  destruct H0 as [v2 [ValsInj12 [SH2 [Minj12 VV2]]]].
-  apply (core_halted23 _ _ _ _ _ _ _ MC23) in SH2; try assumption. 
-  destruct SH2 as [v3 [ValsInj23 [SH3 [MInj23 VV3]]]].
-  exists v3. split. apply (val_inject_compose _ _ _ _ _ ValsInj12 ValsInj23).
-  split. trivial. 
-  split. eapply Mem.inject_compose; eassumption.
-  assumption.
-(*atexternal*)
-  intros. rename st2 into st3. rename m2 into m3. 
-  destruct cd as [[d12 cc2] d23]. 
-  destruct H as [st2 [m2 [j1 [j2 [Y [J [MC12 MC23]]]]]]]. subst.
-  apply (core_at_external12 _ _ _ _ _ _ _ _ _ MC12) in H0; try assumption. 
-  destruct H0 as [MInj12 [PGj1 [vals2 [ValsInj12 [HTVals2 [AtExt2 VV2]]]]]].
-  apply (core_at_external23 _ _ _ _ _ _ _ _ _ MC23) in AtExt2; try assumption. 
-  destruct AtExt2 as [MInj23 [PGj2 [vals3 [ValsInj23 [HTVals3 [AtExt3 VV3]]]]]].
-  split. eapply Mem.inject_compose; eassumption.
-  split. 
-  admit. admit is OK - it's in a comment 
-(*
-Definition meminj_preserves_globals_ind (globals: (block->Prop)*(block->Prop)) f :=
-  (forall b, fst globals b -> f b = Some (b, 0)) /\
-  (forall b, snd globals b -> f b = Some (b, 0)) /\
-  (forall b1 b2 delta, snd globals b2 -> f b1 = Some (b2, delta) -> b1=b2).
-
-need to prove meminj_preserves_globals g1 (compose_meminj j1 j2) 
-          from meminj_preserves_globals g1 j1
-          and meminj_preserves_globals g2 j2*)
-  exists vals3. 
-  split.  eapply forall_val_inject_compose; eassumption.
-  split; try assumption.
-  split; try assumption.
- (*after_external*) clear core_diagram12 core_initial12 core_halted12 
-  core_diagram23 core_initial23 core_halted23. 
-  intros. rename st2 into st3. rename m2 into m3. rename ret2 into ret3. rename m2' into m3'. 
-  destruct cd as [[d12 cc2] d23]. 
-  destruct H0 as [st2 [m2 [j1 [j2 [Y [J [MC12 MC23]]]]]]]. subst.
-  rename H1 into AtExt1. rename H2 into VV1.
-  destruct (core_at_external12 _ _ _ _ _ _ _ _ _ MC12 AtExt1 VV1) 
-   as [MInj12 [PGj1 [vals2 [ValsInj12 [HTVals2 [AtExt2 VV2]]]]]].
-  destruct (core_at_external23 _ _ _ _ _ _ _ _ _ MC23 AtExt2 VV2) 
-   as [MInj23 [PGj2 [vals3 [ValsInj23 [HTVals3 [AtExt3 V3V]]]]]].
-  clear core_at_external12 core_at_external23.
-  assert (HVals1:  Forall2 Val.has_type vals1 (sig_args ef_sig)). 
-  eapply forall_valinject_hastype; eassumption.
-  assert (HRet1: Val.has_type ret1 (proj_sig_res ef_sig)). 
-  eapply valinject_hastype; eassumption.
-  assert (mem_wd m1 /\ mem_wd m2). apply (match_memwd12 _ _ _ _ _ _ MC12). destruct H0 as [WD1 WD2].
-  assert (WD3: mem_wd m3). apply (match_memwd23 _ _ _ _ _ _ MC23).
-  destruct (MEMAX.interpolate_II _ _ _ MInj12 _ H8 _ _ MInj23 _ H10 _ H6 H4 H5 H9 H11 WD1 H13 WD2 WD3 H14)
-    as [m2' [j12' [j23' [X [Incr12 [Incr23 [MInj12' [Fwd2 
-      [MInj23' [Unch22 [Sep12 [Sep23 [Unch222' [Unch2233' WD22']]]]]]]]]]]]]]. 
-  subst.
-  assert (WD2': mem_wd m2'). apply WD22'. apply WD2. 
-  assert (exists ret2, val_inject j12' ret1 ret2 /\ val_inject j23' ret2 ret3 /\
-    Val.has_type ret2 (proj_sig_res ef_sig) /\ val_valid ret2 m2'). 
-  apply val_inject_split in H7. destruct H7 as [ret2 [injRet12 injRet23]]. 
-  exists ret2. split; trivial. split; trivial. 
-  split. eapply valinject_hastype; eassumption.
-  eapply inject_valvalid; eassumption. 
-  destruct H0 as [ret2 [injRet12 [injRet23 [HasTp2 ValV2]]]].
-  assert (Unch111': Mem.unchanged_on (loc_unmapped j1) m1 m1').
-  split; intros; apply H9; unfold compose_meminj, loc_unmapped in *. 
-  rewrite H0. trivial. trivial. 
-  intros. rewrite H0. trivial. trivial.
-  specialize (core_after_external12 _ _ j12' _ _ _ _ _ ret1 m1' m2 m2' ret2 _ MInj12 MC12 AtExt1
-    VV1 PGj1 Incr12 Sep12 MInj12' injRet12 H8 Unch111' Fwd2 Unch22 HasTp2 H13 WD2' H15 ValV2).
-  destruct core_after_external12 as [d12' [c1' [c2' [AftExt1 [AftExt2 MC12']]]]].
-
-  specialize (core_after_external23 _ _ j23' _ _ _ _ vals2 ret2 m2' _ m3' ret3 _ MInj23 MC23 
-    AtExt2 VV2 PGj2 Incr23 Sep23 MInj23' injRet23 Fwd2 Unch222' H10 Unch2233' H12 WD2'
-    H14 ValV2 H16).
-  destruct core_after_external23 as [d23' [cc2' [c3' [AftExt22 [AftExt3 MC23']]]]].
-  rewrite AftExt22 in AftExt2. inv AftExt2.
-  exists (d12', Some c2', d23'). exists c1'. exists c3'.
-  split. assumption.
-  split. assumption.
-  exists c2'. exists m2'. exists j12'. exists j23'. auto.
-Qed.
-  intros.
-  inversion SIM12.
-  intros SIM12.
-  induction SIM12. intros SIM23.
-    apply coop_sim_trans_CaseEq; assumption.
-    apply coop_sim_trans_CaseExt; assumption.
-    apply coop_sim_trans_CaseInj; assumption.
-Qed.
-
-End SM_simulation.
-*)
